sf

SoftwareFoundations/SfLib/Hoare.v
@@ -9,15 +9,114 @@ Require Export Imp.
 Definition Assertion := state -> Prop.
 
 (*
-
-1) The variable X is equal to the integer 3.
-2) The variable X is equal to the metavariable x.
-3) The variable X is less than or equal to the variable Y.
-4) The variable X is equal to 3 or it is less than or equal to the variable Y.
-5) The variable Z squared is less than or equal ot the metavariable x and (Z + 1)^2 is
-   greater than x.
-6) Always holds.
-7) Never holds.
-
+  1) The variable X is equal to the integer 3.
+  2) The variable X is equal to the metavariable x.
+  3) The variable X is less than or equal to the variable Y.
+  4) The variable X is equal to 3 or it is less than or equal to the variable Y.
+  5) The variable Z squared is less than or equal to the metavariable x
+     and (Z + 1)^2 is greater than x.
+  6) The property that always holds. The state can be anything.
+  7) The property that never holds. There does not exists a state that satisfies it.
+     (Note that non-terminating programs do not have a state either.)
 *)
 
+(** Hoare Triples **)
+
+Definition hoare_triple (P : Assertion) (c : com) (Q : Assertion) : Prop :=
+  forall st st', c / st || st' -> P st -> Q st'.
+
+Notation "{{ P }} c {{ Q }}" := (hoare_triple P c Q)
+                                  (at level 90, c at next level) : hoare_spec_scope.
+Open Scope hoare_spec_scope.
+
+(*
+  1) After executing c in any state X will equal 5.
+  2) After executing c in a state where X equals x, X will equal x + 5 in the
+     resulting state.
+  3) After executing c in a state where X <= Y, Y <= X in the resulting state.
+  4) c never terminates (from any starting state).
+  5) Y := X!
+  6) ...
+*)
+
+(*
+  1) valid
+  2) valid
+  3) valid
+  4) valid (vacuously)
+  5) invalid
+  6) valid (vacuously)
+  7) valid (non-termination)
+  8) valid
+  9) valid (non-terminiation)
+*)
+
+Theorem hoare_post_true:
+  forall (P Q : Assertion) c, (forall st, Q st) -> {{P}} c {{Q}}.
+Proof.
+  intros P Q c H. unfold hoare_triple.
+  intros st st' Heval HP.
+  apply H.
+Qed.
+
+Theorem hoare_pre_false:
+  forall (P Q : Assertion) c, (forall st, ~(P st)) -> {{P}} c {{Q}}.
+Proof.
+  intros P Q c H. unfold hoare_triple.
+  intros st st' Heval HP.
+  unfold not in H. apply H in HP.
+  inversion HP.
+Qed.
+
+(** Weakest Preconditions **)
+
+Definition assert_implies (P Q : Assertion) : Prop :=
+  forall st, P st -> Q st.
+
+Notation "P ~~> Q" := (assert_implies P Q) (at level 80).
+Notation "P <~> Q" := (P ~~> Q /\ Q ~~> P) (at level 80).
+
+(*
+  1) X = 5
+  2) Y = y /\ Z = z /\ y + z = 5
+  3) True
+  4) X = 0 => Z = 4 /\ X =/= 0 => W = 3
+  5) False
+  6) True
+*)
+
+Definition is_wp P c Q :=
+  {{P}} c {{Q}} /\ forall P', {{P'}} c {{Q}} -> (forall st, P' st -> P st).
+
+Theorem is_wp_example:
+  is_wp (fun st => st Y <= 4) (X ::= APlus (AId Y) (ANum 1)) (fun st => st X <= 5).
+Proof.
+  unfold is_wp.
+  split.
+    (* => *)
+      unfold hoare_triple. intros.
+      inversion H. subst.
+      unfold update. simpl.
+      assert (forall x y, x <= y -> x + 1 <= S y) by (intros; omega).
+      apply H1. assumption.
+    (* <= *)
+      unfold hoare_triple. intros.
+Admitted. (* FIXME *)
+
+(** Proof Rules **)
+
+(* Assignment *)
+
+Definition assn_sub X a Q : Assertion :=
+  fun (st : state) => Q (update st X (aeval st a)).
+
+Theorem hoare_asgn:
+  forall Q X a, {{assn_sub X a Q}} (X ::= a) {{Q}}.
+Proof.
+  unfold hoare_triple.
+  intros Q X a st st' HE HQ.
+  inversion HE. subst.
+  unfold assn_sub in HQ. assumption.
+Qed.
+
+Example 
